qcp/ast/VC/subst_goal.v
@@ -31,8 +31,8 @@ forall (t_pre: Z) (src_pre: Z) (den_pre: Z) (den_str: (@list Z)) (src_str: (@lis
   &&  ((( &( "t" ) )) # Ptr  |-> t_pre)
   **  ((&((t_pre)  # "term" ->ₛ "type")) # Int  |-> (termtypeID (trm)))
   **  (store_term' t_pre trm )
-  **  ((( &( "src" ) )) # Ptr  |-> src_pre)
   **  ((( &( "den" ) )) # Ptr  |-> den_pre)
+  **  ((( &( "src" ) )) # Ptr  |-> src_pre)
   **  (store_string src_pre src_str )
   **  (store_string den_pre den_str )
 |--
@@ -50,8 +50,8 @@ forall (t_pre: Z) (src_pre: Z) (den_pre: Z) (den_str: (@list Z)) (src_str: (@lis
   &&  ((( &( "t" ) )) # Ptr  |-> t_pre)
   **  ((&((t_pre)  # "term" ->ₛ "type")) # Int  |-> (termtypeID (trm)))
   **  (store_term' t_pre trm )
-  **  ((( &( "src" ) )) # Ptr  |-> src_pre)
   **  ((( &( "den" ) )) # Ptr  |-> den_pre)
+  **  ((( &( "src" ) )) # Ptr  |-> src_pre)
   **  (store_string src_pre src_str )
   **  (store_string den_pre den_str )
 |--
@@ -70,8 +70,8 @@ forall (t_pre: Z) (src_pre: Z) (den_pre: Z) (den_str: (@list Z)) (src_str: (@lis
   &&  ((( &( "t" ) )) # Ptr  |-> t_pre)
   **  ((&((t_pre)  # "term" ->ₛ "type")) # Int  |-> (termtypeID (trm)))
   **  (store_term' t_pre trm )
-  **  ((( &( "src" ) )) # Ptr  |-> src_pre)
   **  ((( &( "den" ) )) # Ptr  |-> den_pre)
+  **  ((( &( "src" ) )) # Ptr  |-> src_pre)
   **  (store_string src_pre src_str )
   **  (store_string den_pre den_str )
 |--
@@ -91,8 +91,8 @@ forall (t_pre: Z) (src_pre: Z) (den_pre: Z) (den_str: (@list Z)) (src_str: (@lis
   &&  ((( &( "t" ) )) # Ptr  |-> t_pre)
   **  ((&((t_pre)  # "term" ->ₛ "type")) # Int  |-> (termtypeID (trm)))
   **  (store_term' t_pre trm )
-  **  ((( &( "src" ) )) # Ptr  |-> src_pre)
   **  ((( &( "den" ) )) # Ptr  |-> den_pre)
+  **  ((( &( "src" ) )) # Ptr  |-> src_pre)
   **  (store_string src_pre src_str )
   **  (store_string den_pre den_str )
 |--
@@ -113,8 +113,8 @@ forall (t_pre: Z) (src_pre: Z) (den_pre: Z) (den_str: (@list Z)) (src_str: (@lis
   &&  ((( &( "t" ) )) # Ptr  |-> t_pre)
   **  ((&((t_pre)  # "term" ->ₛ "type")) # Int  |-> (termtypeID (trm)))
   **  (store_term' t_pre trm )
-  **  ((( &( "src" ) )) # Ptr  |-> src_pre)
   **  ((( &( "den" ) )) # Ptr  |-> den_pre)
+  **  ((( &( "src" ) )) # Ptr  |-> src_pre)
   **  (store_string src_pre src_str )
   **  (store_string den_pre den_str )
 |--
@@ -303,8 +303,8 @@ forall (t_pre: Z) (src_pre: Z) (den_pre: Z) (den_str: (@list Z)) (src_str: (@lis
   &&  ((( &( "t" ) )) # Ptr  |-> t_pre)
   **  ((&((t_pre)  # "term" ->ₛ "type")) # Int  |-> (termtypeID (trm)))
   **  (store_term' t_pre trm )
-  **  ((( &( "src" ) )) # Ptr  |-> src_pre)
   **  ((( &( "den" ) )) # Ptr  |-> den_pre)
+  **  ((( &( "src" ) )) # Ptr  |-> src_pre)
   **  (store_string src_pre src_str )
   **  (store_string den_pre den_str )
 |--
@@ -384,8 +384,8 @@ forall (t_pre: Z) (src_pre: Z) (den_pre: Z) (den_str: (@list Z)) (src_str: (@lis
   **  ((( &( "t" ) )) # Ptr  |-> t_pre)
   **  ((&((t_pre)  # "term" ->ₛ "type")) # Int  |-> (termtypeID (trm)))
   **  ((&((t_pre)  # "term" ->ₛ "content" .ₛ "Var")) # Ptr  |-> y)
-  **  ((( &( "src" ) )) # Ptr  |-> src_pre)
   **  ((( &( "den" ) )) # Ptr  |-> den_pre)
+  **  ((( &( "src" ) )) # Ptr  |-> src_pre)
   **  (store_string den_pre den_str )
 |--
   [| (y <> 0) |]
@@ -469,8 +469,8 @@ forall (t_pre: Z) (src_pre: Z) (den_pre: Z) (den_str: (@list Z)) (src_str: (@lis
   &&  ((( &( "t" ) )) # Ptr  |-> t_pre)
   **  ((&((t_pre)  # "term" ->ₛ "type")) # Int  |-> (termtypeID (trm)))
   **  (store_term' t_pre trm )
-  **  ((( &( "src" ) )) # Ptr  |-> src_pre)
   **  ((( &( "den" ) )) # Ptr  |-> den_pre)
+  **  ((( &( "src" ) )) # Ptr  |-> src_pre)
   **  (store_string src_pre src_str )
   **  (store_string den_pre den_str )
 |--
@@ -519,8 +519,8 @@ forall (t_pre: Z) (src_pre: Z) (den_pre: Z) (den_str: (@list Z)) (src_str: (@lis
   &&  ((( &( "t" ) )) # Ptr  |-> t_pre)
   **  ((&((t_pre)  # "term" ->ₛ "type")) # Int  |-> (termtypeID (trm)))
   **  (store_term' t_pre trm )
-  **  ((( &( "src" ) )) # Ptr  |-> src_pre)
   **  ((( &( "den" ) )) # Ptr  |-> den_pre)
+  **  ((( &( "src" ) )) # Ptr  |-> src_pre)
   **  (store_string src_pre src_str )
   **  (store_string den_pre den_str )
 |--
@@ -576,8 +576,8 @@ forall (t_pre: Z) (src_pre: Z) (den_pre: Z) (den_str: (@list Z)) (src_str: (@lis
   **  ((&((t_pre)  # "term" ->ₛ "content" .ₛ "Apply" .ₛ "right")) # Ptr  |-> z)
   **  (store_term y lt )
   **  (store_term z rt )
-  **  ((( &( "src" ) )) # Ptr  |-> src_pre)
   **  ((( &( "den" ) )) # Ptr  |-> den_pre)
+  **  ((( &( "src" ) )) # Ptr  |-> src_pre)
   **  (store_string src_pre src_str )
   **  (store_string den_pre den_str )
 |--
@@ -648,8 +648,8 @@ forall (t_pre: Z) (src_pre: Z) (den_pre: Z) (den_str: (@list Z)) (src_str: (@lis
   **  ((&((t_pre)  # "term" ->ₛ "content" .ₛ "Apply" .ₛ "left")) # Ptr  |-> retval)
   **  ((&((t_pre)  # "term" ->ₛ "content" .ₛ "Apply" .ₛ "right")) # Ptr  |-> z)
   **  (store_term z rt )
-  **  ((( &( "src" ) )) # Ptr  |-> src_pre)
   **  ((( &( "den" ) )) # Ptr  |-> den_pre)
+  **  ((( &( "src" ) )) # Ptr  |-> src_pre)
 |--
   [| (den_pre <> 0) |] 
   &&  [| (src_pre <> 0) |] 
@@ -713,8 +713,8 @@ forall (t_pre: Z) (src_pre: Z) (den_pre: Z) (den_str: (@list Z)) (src_str: (@lis
   &&  ((( &( "t" ) )) # Ptr  |-> t_pre)
   **  ((&((t_pre)  # "term" ->ₛ "type")) # Int  |-> (termtypeID (trm)))
   **  (store_term' t_pre trm )
-  **  ((( &( "src" ) )) # Ptr  |-> src_pre)
   **  ((( &( "den" ) )) # Ptr  |-> den_pre)
+  **  ((( &( "src" ) )) # Ptr  |-> src_pre)
   **  (store_string src_pre src_str )
   **  (store_string den_pre den_str )
 |--
@@ -818,8 +818,8 @@ forall (t_pre: Z) (src_pre: Z) (den_pre: Z) (den_str: (@list Z)) (src_str: (@lis
   **  ((&((t_pre)  # "term" ->ₛ "content" .ₛ "Quant" .ₛ "var")) # Ptr  |-> y)
   **  ((&((t_pre)  # "term" ->ₛ "content" .ₛ "Quant" .ₛ "body")) # Ptr  |-> z)
   **  (store_term z qterm )
-  **  ((( &( "src" ) )) # Ptr  |-> src_pre)
   **  ((( &( "den" ) )) # Ptr  |-> den_pre)
+  **  ((( &( "src" ) )) # Ptr  |-> src_pre)
   **  (store_string den_pre den_str )
 |--
   [| (den_pre <> 0) |] 
