qcp/ast/VC/thm_apply_goal_check.v
@@ -1,0 +1,6 @@
+Require Import thm_apply_goal thm_apply_proof_auto thm_apply_proof_manual.
+
+Module VC_Correctness : VC_Correct.
+  Include thm_apply_proof_auto.
+  Include thm_apply_proof_manual.
+End VC_Correctness.
