qcp/ast/VC/thm_apply_proof_auto.v
@@ -1,0 +1,104 @@
+Require Import Coq.ZArith.ZArith.
+Require Import Coq.Bool.Bool.
+Require Import Coq.Strings.String.
+Require Import Coq.Lists.List.
+Require Import Coq.Classes.RelationClasses.
+Require Import Coq.Classes.Morphisms.
+Require Import Coq.micromega.Psatz.
+Require Import Coq.Sorting.Permutation.
+From AUXLib Require Import int_auto Axioms Feq Idents List_lemma VMap.
+Require Import SetsClass.SetsClass. Import SetsNotation.
+From SimpleC.SL Require Import Mem SeparationLogic.
+Require Import thm_apply_goal.
+Require Import Logic.LogicGenerator.demo932.Interface.
+Local Open Scope Z_scope.
+Local Open Scope sets.
+Local Open Scope string.
+Local Open Scope list.
+Import naive_C_Rules.
+From SimpleC.EE Require Import ast_lib.
+From SimpleC.EE Require Import malloc.
+From SimpleC.EE Require Import sll_tmpl.
+Local Open Scope sac.
+
+Lemma proof_of_sub_thm_safety_wit_1 : sub_thm_safety_wit_1.
+Proof. Admitted. 
+
+Lemma proof_of_sub_thm_safety_wit_2 : sub_thm_safety_wit_2.
+Proof. Admitted. 
+
+Lemma proof_of_sub_thm_safety_wit_3 : sub_thm_safety_wit_3.
+Proof. Admitted. 
+
+Lemma proof_of_sub_thm_partial_solve_wit_1_pure : sub_thm_partial_solve_wit_1_pure.
+Proof. Admitted. 
+
+Lemma proof_of_sub_thm_partial_solve_wit_1 : sub_thm_partial_solve_wit_1.
+Proof. Admitted. 
+
+Lemma proof_of_sub_thm_partial_solve_wit_2_pure : sub_thm_partial_solve_wit_2_pure.
+Proof. Admitted. 
+
+Lemma proof_of_sub_thm_partial_solve_wit_2 : sub_thm_partial_solve_wit_2.
+Proof. Admitted. 
+
+Lemma proof_of_sub_thm_partial_solve_wit_3 : sub_thm_partial_solve_wit_3.
+Proof. Admitted. 
+
+Lemma proof_of_sub_thm_partial_solve_wit_4 : sub_thm_partial_solve_wit_4.
+Proof. Admitted. 
+
+Lemma proof_of_separate_imply_safety_wit_1 : separate_imply_safety_wit_1.
+Proof. Admitted. 
+
+Lemma proof_of_separate_imply_safety_wit_2 : separate_imply_safety_wit_2.
+Proof. Admitted. 
+
+Lemma proof_of_separate_imply_safety_wit_3 : separate_imply_safety_wit_3.
+Proof. Admitted. 
+
+Lemma proof_of_separate_imply_safety_wit_4 : separate_imply_safety_wit_4.
+Proof. Admitted. 
+
+Lemma proof_of_separate_imply_safety_wit_5 : separate_imply_safety_wit_5.
+Proof. Admitted. 
+
+Lemma proof_of_separate_imply_safety_wit_6 : separate_imply_safety_wit_6.
+Proof. Admitted. 
+
+Lemma proof_of_separate_imply_safety_wit_7 : separate_imply_safety_wit_7.
+Proof. Admitted. 
+
+Lemma proof_of_separate_imply_safety_wit_8 : separate_imply_safety_wit_8.
+Proof. Admitted. 
+
+Lemma proof_of_separate_imply_partial_solve_wit_1 : separate_imply_partial_solve_wit_1.
+Proof. Admitted. 
+
+Lemma proof_of_separate_imply_partial_solve_wit_2_pure : separate_imply_partial_solve_wit_2_pure.
+Proof. Admitted. 
+
+Lemma proof_of_separate_imply_partial_solve_wit_2 : separate_imply_partial_solve_wit_2.
+Proof. Admitted. 
+
+Lemma proof_of_separate_imply_partial_solve_wit_3 : separate_imply_partial_solve_wit_3.
+Proof. Admitted. 
+
+Lemma proof_of_separate_imply_partial_solve_wit_4_pure : separate_imply_partial_solve_wit_4_pure.
+Proof. Admitted. 
+
+Lemma proof_of_separate_imply_partial_solve_wit_4 : separate_imply_partial_solve_wit_4.
+Proof. Admitted. 
+
+Lemma proof_of_separate_imply_partial_solve_wit_5 : separate_imply_partial_solve_wit_5.
+Proof. Admitted. 
+
+Lemma proof_of_separate_imply_partial_solve_wit_6_pure : separate_imply_partial_solve_wit_6_pure.
+Proof. Admitted. 
+
+Lemma proof_of_separate_imply_partial_solve_wit_6 : separate_imply_partial_solve_wit_6.
+Proof. Admitted. 
+
+Lemma proof_of_separate_imply_partial_solve_wit_7 : separate_imply_partial_solve_wit_7.
+Proof. Admitted. 
+
